ts: WIP typeclass all the things

CTL/Basic.lean
@@ -4,47 +4,35 @@ import CTL.Satisfaction
 import CTL.Equivalence
 
 namespace CTL
-open TS
-variable {p : Type}
-
 mutual
-  inductive StateFormula where
-    | top   : StateFormula
-    | prop  : p            → StateFormula
-    | conj  : StateFormula → StateFormula → StateFormula
-    | neg   : StateFormula → StateFormula
-    | exist : PathFormula  → StateFormula
-    | all   : PathFormula  → StateFormula
+  inductive StateFormula (p : Type) where
+    | top   : StateFormula p
+    | prop  : p              → StateFormula p
+    | conj  : StateFormula p → StateFormula p → StateFormula p
+    | neg   : StateFormula p → StateFormula p
+    | exist : PathFormula  p → StateFormula p
+    | all   : PathFormula  p → StateFormula p
 
-  inductive PathFormula where
-    | next : StateFormula → PathFormula
-    | untl : StateFormula → StateFormula → PathFormula
+  inductive PathFormula (p : Type) where
+    | next : StateFormula p → PathFormula p
+    | untl : StateFormula p → StateFormula p → PathFormula p
 end
 
 namespace StateFormula
   open PathFormula
 
-  variable (Φ Φ₁ Φ₂ : @StateFormula p)
+  variable (Φ Φ₁ Φ₂ : StateFormula p)
 
-  @[simp]
-  def bot  : @StateFormula p := neg top
-  @[simp]
-  def disj := neg (conj (neg Φ₁) (neg Φ₂)) -- ⬝¬(⬝¬Φ₁ ⬝∧ ⬝¬Φ₂)
-  @[simp]
-  def impl := disj (neg Φ₁) Φ₂  -- ⬝¬Φ₁ ⬝∨ Φ₂
-  @[simp]
-  def iff  := conj (impl Φ₁ Φ₂) (impl Φ₂ Φ₁)  -- (Φ₁ ⬝→ Φ₂) ⬝∧ (Φ₂ ⬝→ Φ₁)
-  @[simp]
-  def xor  := disj (conj Φ₁ (neg Φ₂)) (conj Φ₂ (neg Φ₁)) -- (Φ₁ ⬝∧ ⬝¬Φ₂) ⬝∨ (Φ₂ ⬝∧ ⬝¬Φ₁)
+  @[simp] def bot  : StateFormula p := neg top
+  @[simp] def disj := neg (conj (neg Φ₁) (neg Φ₂)) -- ⬝¬(⬝¬Φ₁ ⬝∧ ⬝¬Φ₂)
+  @[simp] def impl := disj (neg Φ₁) Φ₂  -- ⬝¬Φ₁ ⬝∨ Φ₂
+  @[simp] def iff  := conj (impl Φ₁ Φ₂) (impl Φ₂ Φ₁)  -- (Φ₁ ⬝→ Φ₂) ⬝∧ (Φ₂ ⬝→ Φ₁)
+  @[simp] def xor  := disj (conj Φ₁ (neg Φ₂)) (conj Φ₂ (neg Φ₁)) -- (Φ₁ ⬝∧ ⬝¬Φ₂) ⬝∨ (Φ₂ ⬝∧ ⬝¬Φ₁)
 
-  @[simp]
-  def potential    := exist (untl top Φ)
-  @[simp]
-  def inevitable   := all (untl top Φ)
-  @[simp]
-  def potentialAll := neg (inevitable (neg Φ))
-  @[simp]
-  def invariant    := neg (potential (neg Φ))
+  @[simp] def potential    := exist (untl top Φ)
+  @[simp] def inevitable   := all (untl top Φ)
+  @[simp] def potentialAll := neg (inevitable (neg Φ))
+  @[simp] def invariant    := neg (potential (neg Φ))
 
 namespace Syntax
   notation  "⬝⊤"   => StateFormula.top
@@ -59,132 +47,139 @@ namespace Syntax
   prefix:50 "⬝∀ "  => StateFormula.all
   prefix:50 "⬝∃♢"  => StateFormula.potential -- \exists\diamondsuit
   prefix:50 "⬝∀♢"  => StateFormula.inevitable -- \forall\diamondsuit
-  prefix:50 "⬝∃■"  => StateFormula.potentialAll -- \exists\sqb
-  prefix:50 "⬝∀■"  => StateFormula.invariant -- \forall\sqb
+  prefix:50 "⬝∃□"  => StateFormula.potentialAll -- \exists\sqw
+  prefix:50 "⬝∀□"  => StateFormula.invariant -- \forall\sqw
   prefix:50 "⬝◯"   => PathFormula.next
   infixr:50 " ⬝U " => PathFormula.untl
 end Syntax
 
 section Satisfaction
-variable {inst : Fintype s}
+variable [Fintype s] [Model p s μ] (m : μ p s)
+
 mutual
   -- s ⊨ Φ
   @[simp]
-  def StateSat (ts : TS s a p) (st : s) :=
-    fun
-      | StateFormula.top => True
-      | ⬝a               => a ∈ ts.label st
-      | ⬝¬Φ              => ¬(StateSat ts st Φ)
-      | Φ₁ ⬝∧ Φ₂         => (StateSat ts st Φ₁) ∧ (StateSat ts st Φ₂)
-      | ⬝∃ φ             => ∃ π : TS.PathFragment.From ts st, PathSat ts π.1.2 φ
-      | ⬝∀ φ             => ∀ π : TS.PathFragment.From ts st, PathSat ts π.1.2 φ
+  def StateSat (Φ : StateFormula p) (st : s) :=
+    match Φ with
+      | ⬝⊤       => True
+      | ⬝a       => a ∈ Model.label m st
+      | ⬝¬Φ      => ¬(StateSat Φ st)
+      | Φ₁ ⬝∧ Φ₂ => (StateSat Φ₁ st) ∧ (StateSat Φ₂ st)
+      | ⬝∃ φ     => ∃ π : Model.Paths m st, PathSat φ π.1
+      | ⬝∀ φ     => ∀ π : Model.Paths m st, PathSat φ π.1
 
   -- π ⊨ φ
   @[simp]
-  def PathSat (ts : TS s a p) (π : ts.PathFragment n) :=
-    fun
-      | ⬝◯ Φ   => StateSat ts (π.second) Φ
-      | Φ ⬝U Ψ => ∃ j : EFin (Order.succ n), (StateSat ts (π.get j) Ψ) ∧ ∀ k : EFin j.val, StateSat ts (π.get (EFin.castLT j.lt k)) Φ
+  def PathSat (φ : PathFormula p) (π : FiniteOrInfinitePathFragment m) :=
+    match φ with
+      | ⬝◯ Φ   => StateSat Φ (PathFragment.second π)
+      | Φ ⬝U Ψ => ∃ j : EFin (Order.succ (PathFragment.length π)), (StateSat Ψ (PathFragment.get π j)) ∧ ∀ k : EFin j.val, StateSat Φ (PathFragment.get π (EFin.castLT j.lt k))
 end
 
-instance : StateSatisfiable p (@StateFormula p) where
-  StateSat := StateSat
+-- @[simp]
+-- theorem StateSat_potentialAll : StateSat m (⬝∃□Φ) st ↔ ∃π : Model.Paths (β := FiniteOrInfinitePathFragment) m st, ∀j, StateSat m Φ (PathFragment.get π.1 j) := by
+  -- simp
 
 @[simp]
-theorem StateSat_potentialAll {st : s} : StateSat ts st (⬝∃■Φ) ↔ ∃π : TS.PathFragment.From ts st, ∀j, StateSat ts (π.1.2.get j) Φ := by
+theorem StateStat_invariant   : StateSat m (⬝∀□Φ) st ↔ ∀π : Model.Paths (β := FiniteOrInfinitePathFragment) m st, ∀j, StateSat m Φ (PathFragment.get π.1 j) := by
   simp
 
-@[simp]
-theorem StateStat_invariant : StateSat ts st (⬝∀■Φ) ↔ ∀π : TS.PathFragment.From ts st, ∀j, StateSat ts (π.1.2.get j) Φ := by
-  simp
+instance : StateSatisfiable StateFormula where
+  StateSat m Φ st := StateSat m Φ st
 end Satisfaction
 
 section Equiv
-variable {Φ Φ' Φ₁ Φ₁' Φ₂ Φ₂' Ψ Ψ' : @StateFormula p}
-
 @[simp]
-theorem conj_congr (h₁ : Equiv (p := p) Φ₁ Φ₁') (h₂ : Equiv (p := p) Φ₂ Φ₂') : Equiv (p := p) (Φ₁ ⬝∧ Φ₂) (Φ₁' ⬝∧ Φ₂') := by
-  simp [Equiv, setOfSatStates, SatState, StateSatisfiable.StateSat, Set.ext_iff] at *
-  intros _ _ _ _ _
+theorem conj_congr (h₁ : Equiv Φ₁ Φ₁') (h₂ : Equiv Φ₂ Φ₂') : Equiv (Φ₁ ⬝∧ Φ₂) (Φ₁' ⬝∧ Φ₂') := by
+  simp only [Equiv, setOfSatStates, SatState, StateSatisfiable.StateSat, StateSat,
+             Set.ext_iff, Subtype.range_coe_subtype, Set.mem_setOf_eq] at *
+  intros _ _ _ _ _ _
   constructor
   . rintro ⟨sat₁, sat₂⟩; constructor; exact (h₁ _).1 sat₁; exact (h₂ _).1 sat₂
   . rintro ⟨sat₁, sat₂⟩; constructor; exact (h₁ _).2 sat₁; exact (h₂ _).2 sat₂
 
 @[simp]
-theorem neg_congr (h : Equiv (p := p) Φ Φ') : Equiv (p := p) (⬝¬Φ) (⬝¬Φ') := by
-  simp [Equiv, setOfSatStates, SatState, StateSatisfiable.StateSat, Set.ext_iff] at *
-  intros _ _ _ _ _
+theorem neg_congr (h : Equiv Φ Φ') : Equiv (⬝¬Φ) (⬝¬Φ') := by
+  simp only [Equiv, setOfSatStates, SatState, StateSatisfiable.StateSat, StateSat,
+             Set.ext_iff, Subtype.range_coe_subtype, Set.mem_setOf_eq] at *
+  intros _ _ _ _ _ _
   constructor
   . rintro negSat sat; exact negSat ((h _).2 sat)
   . rintro negSat sat; exact negSat ((h _).1 sat)
 
 @[simp]
-theorem exist_next_congr (h : Equiv (p := p) Φ Φ') : Equiv (p := p) (⬝∃⬝◯Φ) (⬝∃⬝◯Φ') := by
-  simp [Equiv, setOfSatStates, SatState, StateSatisfiable.StateSat, Set.ext_iff] at *
-  intros _ _ _ _ _
+theorem exist_next_congr (h : Equiv Φ Φ') : Equiv (⬝∃⬝◯Φ) (⬝∃⬝◯Φ') := by
+  simp only [Equiv, setOfSatStates, SatState, StateSatisfiable.StateSat, StateSat, PathSat,
+             Set.ext_iff, Subtype.range_coe_subtype, Set.mem_setOf_eq] at *
+  intros _ _ _ _ _ _
   constructor
   . rintro ⟨π, sat⟩; exact ⟨π, (h _).1 sat⟩
   . rintro ⟨π, sat⟩; exact ⟨π, (h _).2 sat⟩
 
+set_option maxHeartbeats 1000000 in
 @[simp]
-theorem exist_untl_congr (h₁ : Equiv (p := p) Φ Φ') (h₂ : Equiv (p := p) Ψ Ψ') : Equiv (p := p) (⬝∃(Φ ⬝U Ψ)) (⬝∃(Φ' ⬝U Ψ')) := by
-  simp [Equiv, setOfSatStates, SatState, StateSatisfiable.StateSat, Set.ext_iff] at *
-  intros _ _ _ _ _
+theorem exist_untl_congr (h₁ : Equiv Φ Φ') (h₂ : Equiv Ψ Ψ') : Equiv (⬝∃(Φ ⬝U Ψ)) (⬝∃(Φ' ⬝U Ψ')) := by
+  simp only [Equiv, setOfSatStates, SatState, StateSatisfiable.StateSat, StateSat, PathSat,
+             Set.ext_iff, Subtype.range_coe_subtype, Set.mem_setOf_eq] at *
+  intros _ _ _ _ _ _
   constructor
-  . rintro ⟨π, j, ⟨satJ, satK⟩⟩; exact ⟨π, j, ⟨(h₂ _).1 satJ, fun k => (h₁ _).1 (satK k)⟩⟩
-  . rintro ⟨π, j, ⟨satJ, satK⟩⟩; exact ⟨π, j, ⟨(h₂ _).2 satJ, fun k => (h₁ _).2 (satK k)⟩⟩
+  . rintro ⟨π, j, satJ, satK⟩; exact ⟨π, j, (h₂ _).1 satJ, fun k => (h₁ _).1 (satK k)⟩
+  . rintro ⟨π, j, satJ, satK⟩; exact ⟨π, j, (h₂ _).2 satJ, fun k => (h₁ _).2 (satK k)⟩
 
 @[simp]
-theorem all_next_congr (h : Equiv (p := p) Φ Φ') : Equiv (p := p) (⬝∀⬝◯Φ) (⬝∀⬝◯Φ') := by
-  simp [Equiv, setOfSatStates, SatState, StateSatisfiable.StateSat, Set.ext_iff] at *
-  intros _ _ _ _ _
+theorem all_next_congr (h : Equiv Φ Φ') : Equiv (⬝∀⬝◯Φ) (⬝∀⬝◯Φ') := by
+  simp only [Equiv, setOfSatStates, SatState, StateSatisfiable.StateSat, StateSat, PathSat,
+             Set.ext_iff, Subtype.range_coe_subtype, Set.mem_setOf_eq] at *
+  intros _ _ _ _ _ _
   constructor
-  . rintro sat π; rw [← h]; exact sat π
-  . rintro sat π; rw [h]  ; exact sat π
+  . rintro sat π; rw [←h]; exact sat π
+  . rintro sat π; rw [h] ; exact sat π
   done
 
 @[simp]
-theorem all_untl_congr (h₁ : Equiv (p := p) Φ Φ') (h₂ : Equiv (p := p) Ψ Ψ') : Equiv (p := p) (⬝∀(Φ ⬝U Ψ)) (⬝∀(Φ' ⬝U Ψ')) := by
-  simp [Equiv, setOfSatStates, SatState, StateSatisfiable.StateSat, Set.ext_iff] at *
-  intros _ _ _ _ _
+theorem all_untl_congr (h₁ : Equiv Φ Φ') (h₂ : Equiv Ψ Ψ') : Equiv (⬝∀(Φ ⬝U Ψ)) (⬝∀(Φ' ⬝U Ψ')) := by
+  simp only [Equiv, setOfSatStates, SatState, StateSatisfiable.StateSat, StateSat, PathSat,
+             Set.ext_iff, Subtype.range_coe_subtype, Set.mem_setOf_eq] at *
+  intros _ _ _ _ _ _
   constructor
   . rintro sat π; obtain ⟨j, ⟨satJ, satK⟩⟩ := sat π; exact ⟨j, ⟨(h₂ _).1 satJ, fun k => (h₁ _).1 (satK k)⟩⟩
   . rintro sat π; obtain ⟨j, ⟨satJ, satK⟩⟩ := sat π; exact ⟨j, ⟨(h₂ _).2 satJ, fun k => (h₁ _).2 (satK k)⟩⟩
 
-theorem all_next_duality : Equiv (p := p) (⬝∀⬝◯Φ) (⬝¬(⬝∃⬝◯⬝¬Φ)) := by
-  simp [Equiv, setOfSatStates, SatState, StateSatisfiable.StateSat, Set.ext_iff] at *
+theorem all_next_duality : Equiv (⬝∀⬝◯Φ) (⬝¬(⬝∃⬝◯⬝¬Φ)) := by
+  simp [Equiv, setOfSatStates, SatState, StateSatisfiable.StateSat, StateSat, PathSat, Set.ext_iff] at *
 
-theorem inevitable_duality : Equiv (p := p) (⬝∀♢Φ) (⬝¬(⬝∃■⬝¬Φ)) := by
-  simp [Equiv, setOfSatStates, SatState, StateSatisfiable.StateSat, StateFormula.inevitable, PathFormula.untl]
+theorem inevitable_duality : Equiv (⬝∀♢Φ) (⬝¬(⬝∃□⬝¬Φ)) := by
+  simp [Equiv, setOfSatStates, SatState, StateSatisfiable.StateSat, StateSat, PathSat, StateFormula.inevitable, PathFormula.untl] at *
 
-theorem exist_next_duality : Equiv (p := p) (⬝∃⬝◯Φ) (⬝¬(⬝∀⬝◯⬝¬Φ)) := by
+theorem exist_next_duality : Equiv (⬝∃⬝◯Φ) (⬝¬(⬝∀⬝◯⬝¬Φ)) := by
   simp [Equiv, setOfSatStates, SatState, StateSatisfiable.StateSat]
 
-theorem potential_duality : Equiv (p := p) (⬝∃♢Φ) (⬝¬(⬝∀■⬝¬Φ)) := by
+theorem potential_duality : Equiv (⬝∃♢Φ) (⬝¬(⬝∀□⬝¬Φ)) := by
   simp [Equiv, setOfSatStates, SatState, StateSatisfiable.StateSat, StateFormula.potential, PathFormula.untl]
 
-theorem all_untl_duality : Equiv (p := p) (⬝∀(Φ ⬝U Ψ)) (⬝¬(⬝∃(⬝¬Ψ ⬝U (⬝¬Φ ⬝∧ ⬝¬Ψ))) ⬝∧ ⬝¬(⬝∃■⬝¬Ψ)) := by
-  simp [Equiv, setOfSatStates, SatState, StateSatisfiable.StateSat, Set.ext_iff] at *
-  intros _ _ _ _ _
-  constructor
-  . rintro sat
-    constructor
-    . rintro π j negSatΦ negSatΨ
-      obtain ⟨a, ⟨satΨ, satΦ⟩⟩ := sat π
-      sorry
-    . rintro π
-      obtain ⟨_, ⟨_, _⟩⟩ := sat π
-      constructor <;> assumption
-  . rintro ⟨negSat, satΨ⟩ π
-    obtain ⟨j, satΨ'⟩ := satΨ π
-    exact ⟨j, ⟨satΨ', fun k => sorry⟩⟩
-
-theorem all_untl_expansion : Equiv (p := p) (⬝∀(Φ ⬝U Ψ)) (Ψ ⬝∨ (Φ ⬝∧ (⬝∀⬝◯⬝∀(Φ ⬝U Ψ)))) := by
-  -- simp [Equiv, satStateSet, SatState, StateSat, PathSat, StateFormula.disj]
-  -- intro s a ts
-  -- ext x
-  -- done
+theorem all_untl_duality : Equiv (⬝∀(Φ ⬝U Ψ)) (⬝¬(⬝∃(⬝¬Ψ ⬝U (⬝¬Φ ⬝∧ ⬝¬Ψ))) ⬝∧ ⬝¬(⬝∃□⬝¬Ψ)) := by
   sorry
+  -- simp [Equiv, setOfSatStates, SatState, StateSatisfiable.StateSat, Set.ext_iff] at *
+  -- intros _ _ _ _ _
+  -- constructor
+  -- . rintro sat
+    -- constructor
+    -- . rintro π j negSatΦ negSatΨ
+      -- obtain ⟨a, ⟨satΨ, satΦ⟩⟩ := sat π
+      -- sorry
+    -- . rintro π
+      -- obtain ⟨_, ⟨_, _⟩⟩ := sat π
+      -- constructor <;> assumption
+  -- . rintro ⟨negSat, satΨ⟩ π
+    -- obtain ⟨j, satΨ'⟩ := satΨ π
+    -- exact ⟨j, ⟨satΨ', fun k => sorry⟩⟩
+
+theorem all_untl_expansion : Equiv (⬝∀(Φ ⬝U Ψ)) (Ψ ⬝∨ (Φ ⬝∧ (⬝∀⬝◯⬝∀(Φ ⬝U Ψ)))) := by
+  sorry
+  -- -- simp [Equiv, satStateSet, SatState, StateSat, PathSat, StateFormula.disj]
+  -- -- intro s a ts
+  -- -- ext x
+  -- -- done
 
 end Equiv
 end StateFormula
