CTL/Equivalence.lean
@@ -2,42 +2,42 @@ import TS.Basic
 import CTL.Satisfaction
 
 namespace CTL
-variable {p α β : Type}
-         [αSat : StateSatisfiable p α]
-         [βSat : StateSatisfiable p β]
-         (Φ : α)
-         (Ψ : β)
+variable [StateSatisfiable α] [StateSatisfiable β]
+         (Φ : α p) (Ψ : β p)
 
 -- Sat(Φ) = Sat(Ψ)
 @[simp]
 def Equiv :=
-  ∀{s a : Type} {_ : Fintype s}, ∀{ts : TS s a p}, setOfSatStates ts Φ = setOfSatStates ts Ψ
+  ∀ {s} [Fintype s] {μ} [Model p s μ] {m : μ p s}, setOfSatStates m Φ = setOfSatStates m Ψ
 
 -- TS ⊨ Φ ↔ TS ⊨ Ψ
 @[simp]
 def Equiv' :=
-  ∀{s a : Type} {_ : Fintype s}, ∀{ts : TS s a p}, Sat ts Φ ↔ Sat ts Ψ
+  ∀ {s} [Fintype s] {μ} [Model p s μ] {m : μ p s}, Sat m Φ ↔ Sat m Ψ
 
 namespace Equiv
 @[simp]
-theorem equiv'_of_equiv : Equiv (p := p) Φ Ψ → Equiv' (p := p) Φ Ψ := by
-  simp [Equiv, Equiv']
-  intro h _ _ _ _
-  rewrite [h]
-  trivial
+def toEquiv' : Equiv Φ Ψ → Equiv' Φ Ψ := by
+  simp [setOfSatStates, Set.ext_iff]
+  intro h _ _ _ _ _
+  constructor
+  . rintro sat st mem
+    exact (h st).1 (sat st mem)
+  . rintro sat st mem
+    exact (h st).2 (sat st mem)
 
-instance : IsRefl α (Equiv (p := p)) where
+instance : IsRefl (α p) (Equiv) where
   refl := by simp
 
-instance : IsSymm α (Equiv (p := p)) where
+instance : IsSymm (α p) (Equiv) where
   symm := fun Φ Ψ => by simp; intros h _ _ _; exact Eq.symm h
 
-instance : IsTrans α (Equiv (p := p)) where
+instance : IsTrans (α p) (Equiv) where
   trans := fun _ _ _ h₁ h₂ => Trans.trans h₁ h₂
 
-instance : IsPreorder α (Equiv (p := p)) where
+instance : IsPreorder (α p) (Equiv) where
 
-instance : IsEquiv α (Equiv (p := p)) where
+instance : IsEquiv (α p) (Equiv) where
 
 end Equiv
 end CTL
