TS/PathFragment.lean
@@ -5,14 +5,15 @@ import Mathlib.Data.ENat.Basic
 import TS.Basic
 import TS.EFin
 
-class PathFragment {μ : Type} [Model μ] (m : μ) (β : μ → Type) where
+class PathFragment [Fintype s] [Model p s μ] (m : μ p s)
+                   (β : μ p s → Type) where
   length   : (π : β m) → {n : ℕ∞ // Nat.zero < n}
-  get      : (π : β m) → (j : EFin (Order.succ (length π))) → Model.s μ
+  get      : (π : β m) → (j : EFin (Order.succ (length π))) → s
   valid    : (π : β m) → (j : EFin (length π)) → get π j.succ ∈ Model.post m (get π j.castSucc)
 
 namespace PathFragment
-  variable {μ : Type} [Model μ] {m : μ}
-           {β : μ → Type} [PathFragment m β] (π : β m)
+  variable [Fintype s] [Model p s μ] {m : μ p s}
+           {β : μ p s → Type} [PathFragment m β] (π : β m)
 
   @[simp]
   def first := get π EFin.zero
@@ -33,7 +34,7 @@ namespace PathFragment
       exact EFin.inf 1
 
   @[simp]
-  def last? : Option (Model.s μ) := by
+  def last? : Option s := by
     cases h : (length π).val with
     | some n =>
       refine some (get π ?_)
@@ -52,24 +53,22 @@ namespace PathFragment
 end PathFragment
 
 namespace Model
-  variable {μ : Type} [Model μ] (m : μ)
-           {β : μ → Type} [PathFragment m β]
+  variable [Fintype s] [Model p s μ] (m : μ p s)
+           {β : μ p s → Type} [PathFragment m β]
 
   @[simp]
-  def Paths (st : Model.s μ) :=
+  def Paths (st : s) :=
     { π : β m // PathFragment.first π = st ∧ PathFragment.isMaximal π }
 end Model
 
-structure FinitePathFragment {μ : Type} [Model μ] (m : μ) where
+structure FinitePathFragment [Fintype s] [Model p s μ] (m : μ p s) where
   length   : {n : ℕ // 0 < n}
-  states   : Vector (Model.s μ) length.1.succ
-  valid    : ∀ j : Fin length, states.get j.succ ∈ Model.post m (states.get j.castSucc)
+  states   : Vector s length.1.succ
+  valid    : (j : Fin length) → states.get j.succ ∈ Model.post m (states.get j.castSucc)
 
 namespace FinitePathFragment
-  variable {μ : Type} [Model μ] {m : μ}
+  variable [Fintype s] [Model p s μ] {m : μ p s}
            (π : FinitePathFragment m)
-
-  @[simp] def get (j : Fin (length π).1.succ) := π.states.get j
 
   instance : PathFragment m (FinitePathFragment) where
     length π :=
@@ -78,20 +77,19 @@ namespace FinitePathFragment
 
     get π j := by
       cases j with
-      | fin i lt => exact get π ⟨i, lt⟩
+      | fin i lt => exact π.states.get ⟨i, lt⟩
 
     valid π j := by
       cases j with
       | fin i lt => exact valid π ⟨i, lt⟩
-    
 end FinitePathFragment
 
-structure InfinitePathFragment {μ : Type} [Model μ] (m : μ) where
-  states : Stream' (Model.s μ)
-  valid  : ∀ j : ℕ, states.get j.succ ∈ Model.post m (states.get j)
+structure InfinitePathFragment [Fintype s] [Model p s μ] (m : μ p s) where
+  states : Stream' s 
+  valid  : (j : ℕ) → states.get j.succ ∈ Model.post m (states.get j)
 
 namespace InfinitePathFragment
-  variable {μ : Type} [Model μ] {m : μ}
+  variable [Fintype s] [Model p s μ] {m : μ p s}
            (π : InfinitePathFragment m)
 
   @[simp] def get (j : ℕ) := π.states.get j
@@ -107,3 +105,29 @@ namespace InfinitePathFragment
       cases j with
       | inf j => exact valid π j
 end InfinitePathFragment
+
+inductive FiniteOrInfinitePathFragment [Fintype s] [Model p s μ] (m : μ p s) where
+  | fin : FinitePathFragment   m → FiniteOrInfinitePathFragment m
+  | inf : InfinitePathFragment m → FiniteOrInfinitePathFragment m
+
+namespace FiniteOrInfinitePathFragment
+  variable [Fintype s] [Model p s μ] {m : μ p s}
+           (π : FiniteOrInfinitePathFragment m)
+
+  instance : PathFragment m (FiniteOrInfinitePathFragment) where
+    length := fun
+      | .fin π => PathFragment.length π
+      | .inf π => PathFragment.length π
+
+    get := fun
+      | .fin π => PathFragment.get π
+      | .inf π => PathFragment.get π
+
+    valid := fun
+      | .fin π => PathFragment.valid π
+      | .inf π => PathFragment.valid π
+
+  @[simp] def length := PathFragment.length π
+  @[simp] def get := PathFragment.get π
+  @[simp] def valid := PathFragment.valid π
+end FiniteOrInfinitePathFragment
